\begin{definition}[Multifold binomial sum recurrence]
  \begin{align*}
    F_{r} (n, t, j) =
    \begin{cases}
      0, \quad &r<0, \\
      \binom{n-t+j-1}{j}, \quad &r=0, \\
      \sum_{k=1}^{n} F_{r-1}(k, t, j), \quad &r>0.
    \end{cases}
  \end{align*}
\end{definition}

\begin{proposition}[Multifold binomial sum closed form]
  \begin{align*}
    F_{r} (n,t,j)
    = \sum_{k=1}^{n} F_{r-1} (k,t,j)
    = \binom{n-t+j+r-1}{j+r}
    -
    \sum_{s=0}^{r-1} \binom{j-t+(r-1-s)}{j+r-s}
    \KnuthRFoldSum{s}{n}{0}.
  \end{align*}
  \begin{proof}
    Consider the case $r=0$, then result is trivial.
    \begin{align*}
      F_0 (n,t,j) = \binom{n-t+j-1}{j}.
    \end{align*}
    Consider the case $r=1$, then:
    \begin{align*}
      F_1 (n,t,j)
      = \sum_{k=1}^{n} F_0 (k,t,j)
      = \sum_{k=1}^{n} \binom{k-t+j-1}{j}.
    \end{align*}
    By generalized hockey stick identity, closed form
    yields.
    \begin{align*}
      \sum_{k=1}^{n} \binom{k-t+j-1}{j}
      =\sum_{a=j-t}^{n-t+j-1} \binom{a}{j}
      = \binom{n-t+j}{j+1} - \binom{j-t}{j+1}.
    \end{align*}
    Thus,
    \begin{align*}
      F_1 (n,t,j) = \binom{n-t+j}{j+1} - \binom{j-t}{j+1}.
    \end{align*}
    Now we may notice that only the binomial coefficient
    $\binom{n-t+j}{j+1}$ depends on $n$, meaning that
    there is only one place to apply generalized hockey stick
    identity, to get $F_2 (n, t, j)$.
    Hence, for $r=2$, we get,
    \begin{align*}
      F_2 (n,t,j)
      = \sum_{k=1}^{n} F_1 (k,t,j)
      = \sum_{k=1}^{n} \left[ \binom{k-t+j}{j+1} - \binom{j-t}{j+1} \right].
    \end{align*}
    By generalized hockey stick identity
    \begin{align*}
      \sum_{k=1}^{n} \binom{k-t+j}{j+1}
      =\sum_{a=j-t+1}^{n-t+j} \binom{a}{j+1}
      = \binom{n-t+j+1}{j+2} - \binom{j-t+1}{j+2}.
    \end{align*}
    Thus,
    \begin{align*}
      F_2 (n,t,j)
      = \sum_{k=1}^{n} F_1 (k,t,j)
      = \binom{n-t+j+1}{j+2} - \binom{j-t+1}{j+2} - \binom{j-t}{j+1} n.
    \end{align*}
    We actually may observe that $n=\KnuthRFoldSum{1}{n}{0}$,
    and $1=\KnuthRFoldSum{0}{n}{0}$.
    Hence,
    \begin{align*}
      F_2 (n,t,j)
      = \sum_{k=1}^{n} F_1 (k,t,j)
      = \binom{n-t+j+1}{j+2}
      - \binom{j-t+1}{j+2} \KnuthRFoldSum{0}{n}{0}
      - \binom{j-t}{j+1} \KnuthRFoldSum{1}{n}{0}.
    \end{align*}
    By induction over $r$ yields the closed form for $F_r (n,t,j)$.
    \begin{align*}
      F_{r} (n,t,j)
      = \sum_{k=1}^{n} F_{r-1} (k,t,j)
      = \binom{n-t+j+r-1}{j+r}
      -
      \sum_{s=0}^{r-1} \binom{j-t+(r-1-s)}{j+r-s}
      \KnuthRFoldSum{s}{n}{0}.
    \end{align*}
    This completes the proof.
  \end{proof}
\end{proposition}
